pulse/share/steel/examples/pulse/dice/dpe/DPE.fsti
@@ -30,7 +30,6 @@ val ctxt_hndl_t : eqtype
 
 val sid_t : eqtype
 
-// return a session id 
 val open_session (_:unit) : stt (option sid_t) emp (fun _ -> emp)
 
 val destroy_context (sid:sid_t) (ctxt_hndl:ctxt_hndl_t) : stt bool emp (fun _ -> emp)
