pulse/share/steel/examples/pulse/dice/engine/EngineCore.fsti
@@ -1,0 +1,25 @@
+module EngineCore
+open EngineTypes
+open Pulse.Lib.Pervasives
+module A = Pulse.Lib.Array
+module U8 = FStar.UInt8
+module SZ = FStar.SizeT
+open HACL
+
+val l0_is_authentic (repr:engine_record_repr) : prop
+val cdi_functional_correctness (c0:Seq.seq U8.t) (repr:engine_record_repr) : prop 
+
+val engine_main (cdi:cdi_t) (uds:A.larray U8.t (SZ.v uds_len)) (record:engine_record_t)
+                (#p:perm)
+                (#c0:Ghost.erased (elseq U8.t dice_digest_len))
+                (#repr:Ghost.erased engine_record_repr)
+  : stt dice_return_code (A.pts_to uds p uds_bytes **
+                          A.pts_to cdi full_perm c0 **
+                          engine_record_perm record repr)
+                         (fun r -> 
+                            engine_record_perm record repr **
+                            A.pts_to uds p uds_bytes **
+                            exists_ (fun (c1:elseq U8.t dice_digest_len) ->
+                                      A.pts_to cdi full_perm c1 **
+                                      pure (A.is_full_array cdi
+                                        /\ r = DICE_SUCCESS ==> l0_is_authentic repr /\ cdi_functional_correctness c1 repr)))
