pulse/share/steel/examples/pulse/dice/l0/L0Core.fsti
@@ -1,0 +1,136 @@
+module L0Core
+open L0Types
+open Pulse.Lib.Pervasives
+module A = Pulse.Lib.Array
+module U8 = FStar.UInt8
+module SZ = FStar.SizeT
+open HACL
+open X509
+
+// Needs to be exposed so that the caller of l0_main can prove that they
+// computed deviceIDCSR_len correctly
+let deviceIDCSR_pre
+  (deviceIDCSR: deviceIDCSR_ingredients_t) 
+  (deviceIDCRI_len: SZ.t) 
+  (deviceIDCSR_len: SZ.t) 
+  = deviceIDCRI_len == len_of_deviceIDCRI
+                        deviceIDCSR.version
+                        deviceIDCSR.s_common
+                        deviceIDCSR.s_org
+                        deviceIDCSR.s_country /\
+    0 < SZ.v deviceIDCRI_len /\ 
+    valid_deviceIDCSR_ingredients deviceIDCRI_len /\
+    deviceIDCSR_len == length_of_deviceIDCSR deviceIDCRI_len
+
+// Needs to be exposed so that the caller of l0_main can prove that they
+// computed aliasKeyCRT_len correctly
+let aliasKeyCRT_pre
+  (aliasKeyCRT:aliasKeyCRT_ingredients_t) 
+  (aliasKeyTBS_len:SZ.t) 
+  (aliasKeyCRT_len:SZ.t) 
+  = aliasKeyTBS_len == len_of_aliasKeyTBS
+                        aliasKeyCRT.serialNumber
+                        aliasKeyCRT.i_common
+                        aliasKeyCRT.i_org
+                        aliasKeyCRT.i_country
+                        aliasKeyCRT.s_common
+                        aliasKeyCRT.s_org
+                        aliasKeyCRT.s_country
+                        aliasKeyCRT.l0_version /\
+    0 < SZ.v aliasKeyTBS_len /\ 
+    valid_aliasKeyCRT_ingredients aliasKeyTBS_len /\
+    aliasKeyCRT_len == length_of_aliasKeyCRT aliasKeyTBS_len
+
+val aliasKey_post 
+  (alg:alg_t)
+  (dig_len:hkdf_ikm_len)
+  (cdi:Seq.seq U8.t)
+  (fwid:Seq.seq U8.t)
+  (aliasKey_label_len:hkdf_lbl_len)
+  (aliasKey_label:Seq.seq U8.t)
+  (aliasKey_pub:elseq U8.t v32us)
+  (aliasKey_priv:elseq U8.t v32us)
+  : prop
+
+val deviceIDCSR_post
+  (alg:alg_t)
+  (dig_len:hkdf_ikm_len)
+  (cdi: Seq.seq U8.t)
+  (deviceID_label_len: hkdf_lbl_len)
+  (deviceID_label: Seq.seq U8.t)
+  (deviceIDCSR_ingredients: deviceIDCSR_ingredients_t)
+  (deviceIDCSR_len: SZ.t)
+  (deviceIDCSR_buf: elseq U8.t deviceIDCSR_len)
+  : prop
+
+val aliasKeyCRT_post
+  (alg:alg_t)
+  (dig_len:hkdf_ikm_len)
+  (cdi:Seq.seq U8.t)
+  (fwid:Seq.seq U8.t)
+  (deviceID_label_len:hkdf_lbl_len)
+  (deviceID_label:Seq.seq U8.t)
+  (aliasKeyCRT_ingredients:aliasKeyCRT_ingredients_t)
+  (aliasKeyCRT_len:SZ.t)
+  (aliasKeyCRT_buf:elseq U8.t aliasKeyCRT_len)
+  (aliasKey_pub:elseq U8.t v32us)
+  : prop
+
+val l0_main
+  (cdi: A.larray U8.t (SZ.v dice_digest_len))
+  (deviceID_pub: A.larray U8.t (SZ.v v32us))
+  (deviceID_priv: A.larray U8.t (SZ.v v32us))
+  (aliasKey_pub: A.larray U8.t (SZ.v v32us))
+  (aliasKey_priv: A.larray U8.t (SZ.v v32us))
+  (aliasKeyTBS_len:SZ.t)
+  (aliasKeyCRT_len:SZ.t)
+  (aliasKeyCRT: A.larray U8.t (SZ.v aliasKeyCRT_len))
+  (deviceIDCRI_len:SZ.t)
+  (deviceIDCSR_len:SZ.t)
+  (deviceIDCSR: A.larray U8.t (SZ.v deviceIDCSR_len))
+  (record: l0_record_t)
+  (#repr: erased l0_record_repr)
+  (#p:perm)
+  (#cdi0:erased (elseq U8.t dice_digest_len))
+  (#deviceID_pub0 #deviceID_priv0 #aliasKey_pub0 #aliasKey_priv0:erased (elseq U8.t v32us)) 
+  (#aliasKeyCRT0: elseq U8.t aliasKeyCRT_len)
+  (#deviceIDCSR0: elseq U8.t deviceIDCSR_len)
+  : stt unit (l0_record_perm record repr **
+              A.pts_to cdi p cdi0 **
+              A.pts_to deviceID_pub full_perm deviceID_pub0 **
+              A.pts_to deviceID_priv full_perm deviceID_priv0 **
+              A.pts_to aliasKey_pub full_perm aliasKey_pub0 **
+              A.pts_to aliasKey_priv full_perm aliasKey_priv0 **
+              A.pts_to aliasKeyCRT full_perm aliasKeyCRT0 **
+              A.pts_to deviceIDCSR full_perm deviceIDCSR0 **
+              pure (deviceIDCSR_pre record.deviceIDCSR_ingredients deviceIDCRI_len deviceIDCSR_len
+                 /\ aliasKeyCRT_pre record.aliasKeyCRT_ingredients aliasKeyTBS_len aliasKeyCRT_len))
+             (fun _ -> 
+              l0_record_perm record repr **
+              A.pts_to cdi p cdi0 **
+              exists_ (fun (deviceID_pub1:elseq U8.t v32us) ->
+              exists_ (fun (deviceID_priv1:elseq U8.t v32us) -> 
+              exists_ (fun (aliasKey_pub1:elseq U8.t v32us) ->
+              exists_ (fun (aliasKey_priv1:elseq U8.t v32us) ->
+              exists_ (fun (aliasKeyCRT1:elseq U8.t aliasKeyCRT_len) ->
+              exists_ (fun (deviceIDCSR1:elseq U8.t deviceIDCSR_len) ->
+                A.pts_to deviceID_pub full_perm deviceID_pub1 **
+                A.pts_to deviceID_priv full_perm deviceID_priv1 **
+                A.pts_to aliasKey_pub full_perm aliasKey_pub1 **
+                A.pts_to aliasKey_priv full_perm aliasKey_priv1 **
+                A.pts_to aliasKeyCRT full_perm aliasKeyCRT1 **
+                A.pts_to deviceIDCSR full_perm deviceIDCSR1 **
+                pure (
+                  valid_hkdf_ikm_len dice_digest_len /\
+                  aliasKey_post
+                    dice_hash_alg dice_digest_len cdi0 repr.fwid
+                    record.aliasKey_label_len repr.aliasKey_label 
+                    aliasKey_pub1 aliasKey_priv1 /\
+                  deviceIDCSR_post 
+                    dice_hash_alg dice_digest_len cdi0
+                    record.deviceID_label_len repr.deviceID_label record.deviceIDCSR_ingredients 
+                    deviceIDCSR_len deviceIDCSR1 /\       
+                  aliasKeyCRT_post 
+                    dice_hash_alg dice_digest_len cdi0 repr.fwid
+                    record.deviceID_label_len repr.deviceID_label record.aliasKeyCRT_ingredients 
+                    aliasKeyCRT_len aliasKeyCRT1 aliasKey_pub1))))))))
