pulse/share/steel/examples/pulse/dice/l0/L0Crypto.fst
@@ -68,17 +68,18 @@ fn derive_DeviceID'
   (cdi:A.larray U8.t (US.v dice_digest_len))
   (deviceID_label_len:hkdf_lbl_len)
   (deviceID_label:A.larray U8.t (US.v deviceID_label_len))
+  (#p:perm)
   (#cdi0 #deviceID_label0:erased (Seq.seq U8.t))
   (#deviceID_pub0 #deviceID_priv0:erased (elseq U8.t v32us))
   requires (
-    A.pts_to cdi full_perm cdi0 **
+    A.pts_to cdi p cdi0 **
     A.pts_to deviceID_label full_perm deviceID_label0 **
     A.pts_to deviceID_pub full_perm deviceID_pub0 **
     A.pts_to deviceID_priv full_perm deviceID_priv0 **
     pure (valid_hkdf_ikm_len (digest_len alg))
   )
   ensures (
-    A.pts_to cdi full_perm cdi0 **
+    A.pts_to cdi p cdi0 **
     A.pts_to deviceID_label full_perm deviceID_label0 **
     (exists (deviceID_pub1 deviceID_priv1:elseq U8.t v32us). (
         A.pts_to deviceID_pub full_perm deviceID_pub1 **
@@ -113,10 +114,11 @@ fn derive_AliasKey'
   (fwid: A.larray U8.t (US.v v32us))
   (aliasKey_label_len: hkdf_lbl_len)
   (aliasKey_label: A.larray U8.t (US.v aliasKey_label_len))
+  (#p:perm)
   (#cdi0 #fwid0 #aliasKey_label0:erased (Seq.seq U8.t))
   (#aliasKey_pub0 #aliasKey_priv0:erased (elseq U8.t v32us))
   requires (
-    A.pts_to cdi full_perm cdi0 **
+    A.pts_to cdi p cdi0 **
     A.pts_to fwid full_perm fwid0 **
     A.pts_to aliasKey_label full_perm aliasKey_label0 **
     A.pts_to aliasKey_pub full_perm aliasKey_pub0 **
@@ -124,7 +126,7 @@ fn derive_AliasKey'
     pure (is_hashable_len (digest_len alg) /\ valid_hkdf_ikm_len (digest_len alg))
   )
   ensures (
-    A.pts_to cdi full_perm cdi0 **
+    A.pts_to cdi p cdi0 **
     A.pts_to fwid full_perm fwid0 **
     A.pts_to aliasKey_label full_perm aliasKey_label0 **
     (exists (aliasKey_pub1 aliasKey_priv1:elseq U8.t v32us). (
